src/goose_lang/proofmode.v
@@ -286,7 +286,7 @@ Implicit Types z : Z.
 
 Lemma tac_wp_load Δ Δ' s E i K l q v Φ :
   MaybeIntoLaterNEnvs 1 Δ Δ' →
-  envs_lookup i Δ' = Some (false, l ↦{q} v)%I →
+  envs_lookup i Δ' = Some (false, heap_pointsto l q v)%I →
   envs_entails Δ' (WP fill K (Val v) @ s; E {{ Φ }}) →
   envs_entails Δ (WP fill K (Load (LitV l)) @ s; E {{ Φ }}).
 Proof.
@@ -297,7 +297,7 @@ Proof.
 Qed.
 
 Lemma tac_wp_load_persistent Δ s E i K l v Φ :
-  envs_lookup i Δ = Some (true, l ↦□ v)%I →
+  envs_lookup i Δ = Some (true, heap_pointsto l DfracDiscarded v)%I →
   envs_entails Δ (WP fill K (Val v) @ s; E {{ Φ }}) →
   envs_entails Δ (WP fill K (Load (LitV l)) @ s; E {{ Φ }}).
 Proof.
@@ -313,8 +313,8 @@ Qed.
 
 Lemma tac_wp_cmpxchg Δ Δ' Δ'' s E i K l v v1 v2 Φ :
   MaybeIntoLaterNEnvs 1 Δ Δ' →
-  envs_lookup i Δ' = Some (false, l ↦ v)%I →
-  envs_simple_replace i false (Esnoc Enil i (l ↦ v2)) Δ' = Some Δ'' →
+  envs_lookup i Δ' = Some (false, heap_pointsto l (DfracOwn 1) v)%I →
+  envs_simple_replace i false (Esnoc Enil i (heap_pointsto l (DfracOwn 1) v2)) Δ' = Some Δ'' →
   vals_compare_safe v v1 →
   (v = v1 →
    envs_entails Δ'' (WP fill K (Val $ PairV v (LitV $ LitBool true)) @ s; E {{ Φ }})) →
@@ -336,7 +336,7 @@ Qed.
 
 Lemma tac_wp_cmpxchg_fail Δ Δ' s E i K l q v v1 v2 Φ :
   MaybeIntoLaterNEnvs 1 Δ Δ' →
-  envs_lookup i Δ' = Some (false, l ↦{q} v)%I →
+  envs_lookup i Δ' = Some (false, (heap_pointsto l q v))%I →
   v ≠ v1 → vals_compare_safe v v1 →
   envs_entails Δ' (WP fill K (Val $ PairV v (LitV $ LitBool false)) @ s; E {{ Φ }}) →
   envs_entails Δ (WP fill K (CmpXchg (LitV l) v1 v2) @ s; E {{ Φ }}).
@@ -349,8 +349,8 @@ Qed.
 
 Lemma tac_wp_cmpxchg_suc Δ Δ' Δ'' s E i K l v v1 v2 Φ :
   MaybeIntoLaterNEnvs 1 Δ Δ' →
-  envs_lookup i Δ' = Some (false, l ↦ v)%I →
-  envs_simple_replace i false (Esnoc Enil i (l ↦ v2)) Δ' = Some Δ'' →
+  envs_lookup i Δ' = Some (false, heap_pointsto l (DfracOwn 1) v)%I →
+  envs_simple_replace i false (Esnoc Enil i (heap_pointsto l (DfracOwn 1) v2)) Δ' = Some Δ'' →
   v = v1 → vals_compare_safe v v1 →
   envs_entails Δ'' (WP fill K (Val $ PairV v (LitV $ LitBool true)) @ s; E {{ Φ }}) →
   envs_entails Δ (WP fill K (CmpXchg (LitV l) v1 v2) @ s; E {{ Φ }}).
@@ -397,7 +397,7 @@ Tactic Notation "awp_apply" open_constr(lem) "without" constr(Hs) :=
 
 Tactic Notation "wp_untyped_load" :=
   let solve_pointsto _ :=
-    let l := match goal with |- _ = Some (_, (?l ↦{_} _)%I) => l end in
+    let l := match goal with |- _ = Some (_, (heap_pointsto ?l _ _)%I) => l end in
     iAssumptionCore || fail "wp_untyped_load: cannot find" l "↦ ?" in
   wp_pures;
   lazymatch goal with
@@ -418,7 +418,7 @@ Tactic Notation "wp_untyped_load" :=
 
 Tactic Notation "wp_cmpxchg" "as" simple_intropattern(H1) "|" simple_intropattern(H2) :=
   let solve_pointsto _ :=
-    let l := match goal with |- _ = Some (_, (?l ↦{_} _)%I) => l end in
+    let l := match goal with |- _ = Some (_, (heap_pointsto ?l _ _)%I) => l end in
     iAssumptionCore || fail "wp_cmpxchg: cannot find" l "↦ ?" in
   wp_pures;
   lazymatch goal with
@@ -437,7 +437,7 @@ Tactic Notation "wp_cmpxchg" "as" simple_intropattern(H1) "|" simple_intropatter
 
 Tactic Notation "wp_cmpxchg_fail" :=
   let solve_pointsto _ :=
-    let l := match goal with |- _ = Some (_, (?l ↦{_} _)%I) => l end in
+    let l := match goal with |- _ = Some (_, (heap_pointsto ?l _ _)%I) => l end in
     iAssumptionCore || fail "wp_cmpxchg_fail: cannot find" l "↦ ?" in
   wp_pures;
   lazymatch goal with
@@ -455,7 +455,7 @@ Tactic Notation "wp_cmpxchg_fail" :=
 
 Tactic Notation "wp_cmpxchg_suc" :=
   let solve_pointsto _ :=
-    let l := match goal with |- _ = Some (_, (?l ↦{_} _)%I) => l end in
+    let l := match goal with |- _ = Some (_, (heap_pointsto ?l _ _)%I) => l end in
     iAssumptionCore || fail "wp_cmpxchg_suc: cannot find" l "↦ ?" in
   wp_pures;
   lazymatch goal with
